



Modularity)

$$Q = \frac{1}{2m} \sum_{ij} \left(A_{ij} - \frac{k_i k_j}{2m} \right) \delta_{c(i)c(j)}$$

k = # of edges attached

A = adjacency matrix

m = # of edges

$$1, 3 \Rightarrow \left(1 - \frac{2 \times 3}{14} \right) (1) = \left(1 - \frac{3}{7} \right) = \frac{4}{7}$$

$$1, 2 \Rightarrow \left(1 - \frac{2 \times 2}{14} \right) (1) = \frac{5}{7}$$

$$3, 2 \Rightarrow \left(1 - \frac{2 \times 3}{14} \right) (1) = \frac{4}{7}$$

$\left. \begin{matrix} \frac{4}{7} \\ \frac{5}{7} \\ \frac{4}{7} \end{matrix} \right\} \frac{13}{7}$

$$1, 4 \Rightarrow 0 \quad 1, 6 \Rightarrow 0$$

$$3, 4 \Rightarrow 0 \quad 2, 6 \Rightarrow 0$$

$$2, 4 \Rightarrow 0 \quad 3, 6 \Rightarrow 0$$

$$1, 5 \Rightarrow 0$$

$$2, 5 \Rightarrow 0 \quad \frac{1}{14} \left(\frac{13}{7} + \frac{13}{7} - \frac{17}{7} \right) = \frac{9}{98}$$

$$3, 5 \Rightarrow 0$$

$$4, 5 \Rightarrow \left(1 - \frac{3 \times 2}{14} \right) (1) = \left(1 - \frac{3}{7} \right) = \frac{4}{7}$$

$$4, 6 \Rightarrow \left(1 - \frac{3 \times 2}{14} \right) (1) = \frac{4}{7}$$

$$5, 6 \Rightarrow \left(1 - \frac{2 \times 2}{14} \right) (1) = \frac{5}{7}$$

$$\frac{13}{7}$$

$$6, 6 \Rightarrow \left(0 - \frac{2 \times 2}{14} \right) (1) = -\frac{2}{7}$$

$$5, 5 \Rightarrow \left(0 - \frac{2 \times 2}{14} \right) (1) = -\frac{2}{7}$$

$$4, 4 \Rightarrow \left(0 - \frac{3 \times 3}{14} \right) (1) = -\frac{4.5}{7}$$

$$3, 3 \Rightarrow \left(0 - \frac{3 \times 3}{14} \right) (1) = -\frac{4.5}{7}$$

$$-\frac{17}{7}$$

$$2, 2 \Rightarrow \left(0 - \frac{2 \times 2}{14}\right)(1) = -\frac{2}{7}$$

$$1, 1 \Rightarrow \left(0 - \frac{2 \times 2}{14}\right)(1) = -\frac{2}{7}$$